Addressing issue 8.
The objective of this set of changes is to ensure we only have one
data-type which represents a program (Prog). Encoding/decoding goes
directly
there. There is no longer two different APIs (one for "machines" and
another for programs) and instead only one unified API (only programs).

src/LangDec.v
@@ -3,65 +3,60 @@ Require Import Coq.Bool.Bool.
 
 Section Defs.
   Definition A_tm : lang := fun p =>
-    let (M, w) := decode_machine_input p in
-    Exec M w Accept.
+    let (M, w) := decode_prog_input p in
+    Run M w Accept.
 
   (** If [d] recognizes A_tm and machine d runs <M,w> *)
-  Local Lemma a_tm_run_reject:
+  Lemma a_tm_run_reject:
     forall d,
     Recognizes d A_tm ->
     forall w M,
-    Exec d (encode_machine_input M w) Reject -> 
-    forall r,
-    Exec M w r ->
-    r <> Accept.
+    Run d (encode_prog_input M w) Reject -> 
+    ~ Run M w Accept.
   Proof.
     intros.
     intros N.
     apply recognizes_run_reject with (L:=A_tm) in H0; auto.
     unfold A_tm in H0.
-    rewrite decode_encode_machine_input_rw in *.
-    subst.
+    run_simpl_all.
     contradiction.
   Qed.
 
-  Local Lemma a_tm_run_loop:
+  Lemma a_tm_run_loop:
     forall d,
     Recognizes d A_tm ->
     forall w m,
-    Exec d (encode_machine_input m w) Loop -> 
-    forall r,
-    Exec m w r ->
-    r <> Accept.
+    Run d (encode_prog_input m w) Loop -> 
+    ~ Run m w Accept.
   Proof.
     intros.
     intros N; subst.
     apply recognizes_run_loop with (L:=A_tm) in H0; auto.
     unfold A_tm in H0.
-    rewrite decode_encode_machine_input_rw in *.
+    rewrite decode_encode_prog_input_rw in *.
     contradiction.
   Qed.
 
-  Local Lemma a_tm_run_accept:
+  Lemma a_tm_run_accept:
     forall d,
     Recognizes d A_tm ->
     forall w m,
-    Exec d (encode_machine_input m w) Accept -> 
-    Exec m w Accept.
+    Run d (encode_prog_input m w) Accept -> 
+    Run m w Accept.
   Proof.
     intros.
     apply recognizes_run_accept with (L:=A_tm) in H0; auto.
     unfold A_tm in *.
-    rewrite decode_encode_machine_input_rw in *.
+    run_simpl_all.
     assumption.
   Qed.
 
   (* -------------------------------------------------------------------------- *)
 
-  Definition Negator (D:machine) :=
+  Definition Negator (D:Prog) : lang :=
     fun p =>
-      let M := decode_machine p in
-      Exec D (encode_machine_input M p) Reject.
+      let M := decode_prog p in
+      Run D (encode_prog_input M p) Reject.
 
   (** [D] recognizes [A_tm].
       N accepts <M>, which means that D rejects <M, <M>>.
@@ -72,8 +67,8 @@ Section Defs.
   Lemma decider_not_reject:
     forall m i,
     Decider m ->
-    ~ Exec m i Reject ->
-    Exec m i Accept.
+    ~ Run m i Reject ->
+    Run m i Accept.
   Proof.
     intros.
     edestruct decider_to_run; eauto.
@@ -83,8 +78,8 @@ Section Defs.
   Lemma decider_not_accept:
     forall m i,
     Decider m ->
-    ~ Exec m i Accept ->
-    Exec m i Reject.
+    ~ Run m i Accept ->
+    Run m i Reject.
   Proof.
     intros.
     edestruct decider_to_run; eauto.
@@ -95,27 +90,25 @@ Section Defs.
     forall N D w,
     Recognizes D A_tm ->
     Recognizes N (Negator D) ->
-    Exec N w Accept ->
-    forall r,
-    Exec (decode_machine w) w r ->
-    r <> Accept.
+    Run N w Accept ->
+    ~ Run (decode_prog w) w Accept.
   Proof.
     intros.
     apply recognizes_run_accept with (L:=Negator D) in H1; auto.
-    eapply a_tm_run_reject in H2; eauto.
+    eapply a_tm_run_reject in H1; eauto.
   Qed.
 
   Lemma negator_no:
     forall D w,
     Decider D ->
     ~ Negator D w ->
-    Exec D <[ decode_machine w, w ]> Accept.
+    Run D <[ decode_prog w, w ]> Accept.
   Proof.
     intros.
     unfold Negator in H0.
-    remember (encode_machine_input (decode_machine w) w) as j.
+    remember (encode_prog_input (decode_prog w) w) as j.
     (* If D does not reject, it must accept *)
-    assert (Hd: Exec D j Accept) by eauto using decider_not_reject.
+    assert (Hd: Run D j Accept) by eauto using decider_not_reject.
     subst.
     assumption.
   Qed.
@@ -124,13 +117,13 @@ Section Defs.
     forall N D w,
     Recognizes D A_tm ->
     Recognizes N (Negator D) ->
-    Exec N w Reject ->
+    Run N w Reject ->
     Decider D ->
-    Exec (decode_machine w) w Accept.
+    Run (decode_prog w) w Accept.
   Proof.
     intros.
     apply recognizes_run_reject with (L:=Negator D) in H1; auto.
-    assert (Ha: Exec D <[ decode_machine w, w ]> Accept) by auto using negator_no.
+    assert (Ha: Run D <[ decode_prog w, w ]> Accept) by auto using negator_no.
     apply a_tm_run_accept in Ha; auto.
   Qed.
 
@@ -138,9 +131,9 @@ Section Defs.
     forall N D w,
     Recognizes D A_tm ->
     Recognizes N (Negator D) ->
-    Exec N w Loop ->
+    Run N w Loop ->
     Decider D ->
-    Exec (decode_machine w) w Accept.
+    Run (decode_prog w) w Accept.
   Proof.
     intros.
     apply recognizes_run_loop with (L:=Negator D) in H1; auto.
@@ -159,31 +152,36 @@ Section Defs.
           2. Output the opposite of what D outputs. That is, if D accepts,
             reject ; and if D rejects, accept.”
   *)
-  Definition negator D w :=
-    let M := decode_machine w in
-    (* D decides A_TM, thus we are running M with <M> *)
-    mlet b <- Call D <[ M , w ]> in
-    halt_with (negb b).
+  Definition negator (D:Prog) :=
+    Read (fun w =>
+      let M := decode_prog w in
+      (* D decides A_TM, thus we are running M with <M> *)
+      With <[ M , w ]> (
+        mlet b <- D in
+        halt_with (negb b)
+      )
+    ).
 
-  Local Lemma negator_recognizes:
+  Lemma negator_recognizes:
     forall H,
-    Recognizes (Build (negator H)) (Negator H).
+    Recognizes (negator H) (Negator H).
   Proof.
     intros.
     unfold Recognizes.
     split; intros. {
       unfold negator, Negator in *.
-      run_simpl_all.
       inversion H0; subst; clear H0.
+      inversion H2; subst; clear H2.
+      inversion H5; subst; clear H5.
       run_simpl_all.
       assumption.
     }
     unfold Negator in *.
-    run_simpl_all.
     unfold negator.
+    constructor.
+    constructor.
     apply run_seq_reject.
-    - apply run_call.
-      assumption.
+    - assumption.
     - apply run_ret.
   Qed.
 
@@ -197,24 +195,21 @@ Section Defs.
     destruct N as (D, is_dec).
     (* Now we construct a new Turing machine [negator] with D as a subroutine. *)
     assert (X:= negator_recognizes D).
-    remember (Build (negator D)) as N.
+    remember (negator D) as N.
     destruct is_dec as (Hrec, Hdec).
     (* What happens when we run [negator] with its own description <negator> as
       input? *)
-    destruct (exec_exists N (encode_machine N)) as (r, He).
+    destruct (run_exists N (encode_prog N)) as (r, He).
     assert (Hx := He).
     (* (Let us duplicate Heqr as we will need it later.) *)
     destruct r; subst.
     - eapply run_negator_accept with (D:=D) in He; eauto.
-      rewrite decode_encode_machine_rw in *; auto.
+      run_simpl_all.
+      contradiction.
     - apply run_negator_reject with (D:=D) in He; eauto.
-      rewrite decode_encode_machine_rw in *.
-      assert (N: Reject = Accept) by eauto using exec_fun.
-      inversion N.
+      run_simpl_all.
     - apply run_negator_loop with (D:=D) in He; eauto.
-      rewrite decode_encode_machine_rw in *.
-      assert (N: Loop = Accept) by eauto using exec_fun.
-      inversion N.
+      run_simpl_all.
   Qed.
 
   (** Theorem 4.11, pp 207 *)
@@ -234,10 +229,11 @@ Section Defs.
 
   (* -------------------------------------------------------------------------- *)
 
-  Local Definition A_tm_mach : machine :=
-    Build (fun p => 
-      let (M, w) := decode_machine_input p in
-      Call M w).
+  Definition A_tm_mach : Prog :=
+    Read (fun p => 
+      let (M, w) := decode_prog_input p in
+      With w M
+    ).
 
   Lemma accept_to_a_tm:
     forall M L w,
@@ -247,7 +243,7 @@ Section Defs.
   Proof.
     intros.
     unfold A_tm.
-    destruct (decode_machine_input _) as (M', w') eqn:Hr.
+    destruct (decode_prog_input _) as (M', w') eqn:Hr.
     run_simpl.
     inversion Hr; subst; clear Hr.
     apply recognizes_accept with (L:=L); auto.
@@ -261,10 +257,10 @@ Section Defs.
   Proof.
     intros.
     unfold A_tm in *.
-    destruct (decode_machine_input _) as (M', w') eqn:Hr.
+    destruct (decode_prog_input _) as (M', w') eqn:Hr.
     run_simpl.
     inversion Hr; subst; clear Hr.
-    apply recognizes_run_accept with (m:=M'); auto.
+    eapply recognizes_run_accept; eauto.
   Qed.
 
   Lemma a_tm_accept_iff:
@@ -278,21 +274,21 @@ Section Defs.
     - apply accept_to_a_tm; auto.
   Qed.
 
-  Local Lemma a_tm_recognizes:
+  Lemma a_tm_recognizes:
     Recognizes A_tm_mach A_tm.
   Proof.
     intros.
     unfold Recognizes.
     unfold A_tm_mach, A_tm.
     split; intros. {
-      run_simpl_all.
-      destruct (decode_machine_input i) as (m, w).
-      run_simpl.
+      inversion H; subst; clear H.
+      destruct (decode_prog_input i) as (m, w).
+      inversion H1; subst; clear H1.
       assumption.
     }
-    run_simpl.
-    destruct (decode_machine_input i) as (m, w).
-    apply run_call.
+    constructor.
+    destruct (decode_prog_input i) as (m, w).
+    constructor.
     assumption.
   Qed.
 
@@ -304,11 +300,11 @@ Section Defs.
 
   (* -------------------------------------------------------------------------- *)
 
-  Definition Inv (m:machine) := fun i => Exec m i Reject.
+  Definition Inv (m:Prog) := fun i => Run m i Reject.
 
-  Definition InvM (n m:machine) := forall i r1 r2,
-    Exec m i r1 ->
-    Exec n i r2 ->
+  Definition InvM (n m:Prog) := forall i r1 r2,
+    Run m i r1 ->
+    Run n i r2 ->
     neg r1 = r2.
 
   Lemma neg_dec:
@@ -328,28 +324,33 @@ Section Defs.
     Recognizes n (Inv m) /\ InvM n m.
   Proof.
     intros.
-    exists (Build (fun w => (Seq (Call m w) (fun b => halt_with (negb b) )))).
+    exists (
+      Read (
+        fun w =>
+          mlet b <- m in
+          halt_with (negb b)
+        )
+    ).
     split. {
       unfold Recognizes.
       split; intros; unfold Inv in *; run_simpl_all.
-      - inversion H0; subst; clear H0.
+      - inversion H2; subst; clear H2.
         run_simpl_all.
         assumption.
-      - apply run_seq_reject.
-        + apply run_call.
-          assumption.
+      - constructor.
+        apply run_seq_reject.
+        + assumption.
         + apply run_ret.
     }
     unfold InvM.
     intros.
-    run_simpl.
-    inversion H1; subst; clear H1;
-    run_simpl_all.
+    inversion H1; subst; clear H1.
+    inversion H3; subst; clear H3; run_simpl_all.
     - eauto using neg_dec.
     - reflexivity.
   Qed.
 
-  Local Lemma inv_compl_equiv:
+  Lemma inv_compl_equiv:
     forall m L,
     Decides m L ->
     Equiv (Inv m) (compl L).
@@ -360,7 +361,7 @@ Section Defs.
     eauto using decides_run_reject, decides_reject.
   Qed.
 
-  Local Lemma recognizes_inv_compl:
+  Lemma recognizes_inv_compl:
     forall m n L,
     Decides m L ->
     Recognizes n (Inv m) ->
@@ -388,9 +389,8 @@ Section Defs.
     apply recognizes_inv_compl with (L:=L) in H0; auto.
     apply decides_def.
     * assumption.
-    * unfold Decider; intros.
-      intros Hn; subst.
-      destruct (exec_exists m i) as (r, He).
+    * intros i Hn.
+      destruct (run_exists m i) as (r, He).
       unfold InvM in *.
       assert (r = Loop). {
         assert (Hx: neg r = Loop) by eauto.
@@ -413,47 +413,37 @@ Section Defs.
     + apply decides_to_compl with (m:=m) (N:=N); auto.
   Qed.
 
-  Definition par_run (m1 m2 m3:machine) :=
+  Definition par_run (m1 m2:Prog) p :=
     forall i,
       (
-        Exec m3 i Accept /\ Exec m1 i Accept
+        Run p i Accept /\ Run m1 i Accept
       ) \/ (
-        Exec m3 i Reject /\ (Exec m1 i Reject \/ ~ Exec m2 i Loop)
+        Run p i Reject /\ (Run m1 i Reject \/ ~ Run m2 i Loop)
       ) \/ (
-        Exec m3 i Loop /\ Exec m1 i Loop /\ Exec m2 i Loop
+        Run p i Loop /\ Run m1 i Loop /\ Run m2 i Loop
       ).
 
-  Definition par_mach M1 M2 (w: input) : Prog :=
-      plet b <- Call M1 w \\ Call M2 w in
+  Definition par_mach M1 M2 : Prog :=
+    Read (fun w =>
+      plet b <- M1 \\ M2 in
       match b with
       | pleft true
       | pboth true _ => ACCEPT
       | pright false => ACCEPT
       | _ => REJECT
       end
-  .
-(*
-  Lemma lang_accept_rev:
-    forall m w,
-    Exec m w Accept ->
-    Lang m w.
-  Proof.
-    intros.
-    unfold Lang.
-    symmetry.
-    assumption.
-  Qed.
-*)
+    ).
+
   Lemma run_par_both_eq:
-    forall p1 p2 (k:par_result -> Prog) r1 r2 b1 b2 r,
-    Run p1 r1 ->
-    Run p2 r2 ->
+    forall i p1 p2 (k:par_result -> Prog) r1 r2 b1 b2 r,
+    Run p1 i r1 ->
+    Run p2 i r2 ->
     Dec r1 b1 ->
     Dec r2 b2 ->
-    Run (k (pboth b1 b2)) r ->
-    Run (k (pleft b1)) r ->
-    Run (k (pright b2)) r ->
-    Run (Par p1 p2 k) r.
+    Run (k (pboth b1 b2)) i r ->
+    Run (k (pleft b1)) i r ->
+    Run (k (pright b2)) i r ->
+    Run (Par p1 p2 k) i r.
   Proof.
     intros.
     apply run_par_both with (r1:=r1) (r2:=r2) (b1:=b1) (b2:=b2); auto.
@@ -473,12 +463,12 @@ Section Defs.
 
   Lemma par_mach_lang:
     forall m1 m2,
-    (forall i r1 r2, Exec m1 i r1 -> Exec m2 i r2 -> DisjointResults r1 r2) ->
-    PRecognizes (par_mach m1 m2) (Lang m1).
+    (forall i r1 r2, Run m1 i r1 -> Run m2 i r2 -> DisjointResults r1 r2) ->
+    Recognizes (par_mach m1 m2) (fun i => Run m1 i Accept).
   Proof.
     unfold par_mach.
     intros m1 m2 Hr; intros.
-    apply p_recognizes_def.
+    apply recognizes_def.
     + intros.
       (* Show that whenever the implementation accepts, then the language
          accepts. We do this by thinking about the execution top to bottom:
@@ -486,7 +476,8 @@ Section Defs.
          *)
       (* We perform an inversion on assumption H, which will return a case per
          constructor for par, since the first instructio nis a parallel call. *)
-      inversion H; subst; clear H; run_simpl_all; auto.
+      inversion H; subst; clear H.
+      inversion H1; subst; clear H1; run_simpl_all.
       * (* Case par_l_seq: m1 terminated*)
         (* If m1 terminates, then we have:
           Run (if b then ACCEPT else REJECT) Accept
@@ -519,35 +510,34 @@ Section Defs.
           assert (Hd: DisjointResults Reject Reject) by eauto.
           inversion Hd.
     + intros.
-      destruct (exec_exists m2 i) as (r, He).
-      apply run_call in H.
-      apply run_call in He.
+      destruct (run_exists m2 i) as (r, He).
+      constructor.
       destruct r.
       * (* Absurd case: both cannot accept *)
         run_simpl_all.
         assert (N: DisjointResults Accept Accept) by eauto.
         inversion N.
       * apply run_par_both_eq with (r1:=Accept) (r2:=Reject) (b1:=true) (b2:=false);
-        auto using dec_accept, dec_reject, run_ret.
-      * apply run_par_l_accept; auto using run_ret.
+        auto using dec_accept, dec_reject, run_ret, run_call.
+      * apply run_par_l_accept; auto using run_ret, run_call.
   Qed.
 
   Lemma par_run_spec:
     forall m1 m2,
-    (forall i r1 r2, Exec m1 i r1 -> Exec m2 i r2 -> DisjointResults r1 r2) ->
-    par_run m1 m2 (Build (par_mach m1 m2)).
+    (forall i r1 r2, Run m1 i r1 -> Run m2 i r2 -> DisjointResults r1 r2) ->
+    par_run m1 m2 (par_mach m1 m2).
   Proof.
     intros m1 m3 Hr.
     unfold par_run.
     unfold par_mach in *.
     intros.
-    remember (Build _) as m.
-    destruct (exec_exists m i) as (r, He).
+    remember (Read _) as p.
+    destruct (run_exists p i) as (r, He).
     destruct r.
     - left; split; auto.
       subst.
-      run_simpl.
       inversion He; subst; clear He.
+      inversion H0; subst; clear H0.
       + destruct b; run_simpl_all.
         assumption.
       + destruct b; run_simpl_all.
@@ -557,13 +547,14 @@ Section Defs.
         apply par_choice_spec in Hp;
         inversion Hp; subst; clear Hp;
         destruct b; run_simpl_all; auto.
-        inversion H4; subst; clear H4; auto.
+        inversion H5; subst; clear H5; auto.
         assert (N: DisjointResults Reject Reject) by eauto.
         inversion N.
     - right.
       left. split; auto.
-      subst; run_simpl.
-      inversion He; subst; clear He;
+      subst.
+      inversion He; subst; clear He.
+      inversion H0; subst; clear H0;
       try (destruct b; run_simpl_all; auto).
       + right.
         intros N.
@@ -573,14 +564,15 @@ Section Defs.
         apply par_choice_spec in Hp;
         inversion Hp; subst; clear Hp;
         destruct b; run_simpl_all; auto.
-        inversion H4; subst; clear H4; auto.
+        inversion H5; subst; clear H5; auto. (* Dec r1 b1 *)
         assert (N: DisjointResults Accept Accept) by eauto.
         inversion N.
     - right.
       right.
       split; auto.
-      subst; run_simpl.
-      inversion He; subst; clear He;
+      subst.
+      inversion He; subst; clear He.
+      inversion H0; subst; clear H0;
       try (destruct b; run_simpl_all; auto).
       + destruct (par_choice _ _ _ _) eqn:Hp;
         apply par_choice_spec in Hp;
@@ -593,15 +585,14 @@ Section Defs.
 
   Lemma par_run_exists:
     forall m1 m2,
-    (forall i r1 r2, Exec m1 i r1 -> Exec m2 i r2 -> DisjointResults r1 r2) ->
-    exists m3,
-      Recognizes m3 (Lang m1) /\ par_run m1 m2 m3.
+    (forall i r1 r2, Run m1 i r1 -> Run m2 i r2 -> DisjointResults r1 r2) ->
+    exists p,
+      Recognizes p (fun i => Run m1 i Accept) /\ par_run m1 m2 p.
   Proof.
     intros.
-    exists (Build (par_mach m1 m2)).
+    exists (par_mach m1 m2).
     split.
-    - rewrite <- p_recognizes_rw.
-      auto using par_mach_lang.
+    - auto using par_mach_lang.
     - auto using par_run_spec.
   Qed.
 
@@ -621,8 +612,8 @@ Section Defs.
     Recognizes m1 L ->
     Recognizes m2 (compl L) ->
     forall i,
-    Exec m1 i Reject ->
-    Exec m2 i Accept.
+    Run m1 i Reject ->
+    Run m2 i Accept.
   Proof.
     intros.
     apply recognizes_run_reject with (L:=L) in H1; auto.
@@ -633,7 +624,7 @@ Section Defs.
     forall m1 m2 L,
     Recognizes m1 L ->
     Recognizes m2 (compl L) ->
-    (forall i r1 r2, Exec m1 i r1 -> Exec m2 i r2 -> DisjointResults r1 r2).
+    (forall i r1 r2, Run m1 i r1 -> Run m2 i r2 -> DisjointResults r1 r2).
   Proof.
     intros.
     destruct r1.
@@ -659,26 +650,27 @@ Section Defs.
     intros.
     destruct H as (m1, H).
     destruct H0 as (m2, H0).
-    destruct par_run_exists with (m1:=m1) (m2:=m2) as (mpar, (Hr,Hp));
-    eauto using recognizes_co_recognizes_disjoint.
+    destruct par_run_exists with (m1:=m1) (m2:=m2) as (mpar, (Hr,Hp)). {
+      intros.
+      run_simpl_all.
+      eapply recognizes_co_recognizes_disjoint with (m1:=m1) (m2:=m2); eauto.
+    }
     apply decidable_def with (m:=mpar).
     apply decides_def.
     + unfold Recognizes.
       intros.
       rewrite (Hr i).
       rewrite (H i).
-      intuition.
+      reflexivity.
     + unfold Decider.
       intros.
       assert (Hp := Hp i).
-      destruct (exec_exists m1 i) as (r', He).
+      destruct (run_exists m1 i) as (r', He).
       intros N; subst.
       destruct r'.
       - unfold Lang in *.
-        assert (Hr := Hr i).
-        rewrite <- Hr in He.
-        assert (N: Loop = Accept) by (run_simpl; auto).
-        inversion N.
+        repeat rewrite build_spec in *.
+        intuition; run_simpl_all.
       - apply reject_recognize_to_accept_co_recognize with (m2:=m2) (L:=L) in He; auto.
         intuition; run_simpl_all.
       - (* Since [m1 i] loops, then [m2 i] accepts : *)
