src/Turing.v
@@ -10,26 +10,6 @@ Require Import Coq.Logic.Classical_Prop.
   Parameter input_eq_dec: forall x y: input, {x = y} + {x <> y}.
   Parameter machine: Type.
 
-  (** We also define a function to serialize a machine into a string (of type
-      input). In the book, this corresponds to notation <M>. *)
-  Parameter encode_machine: machine -> input.
-  (** Similarly, we have a function that takes a string and produces a machine.
-      In the book, this corresponds to notation M = <M> *)
-  Parameter decode_machine: input -> machine.
-  (** Decoding and encoding a machine yields the same machine. *)
-  Axiom decode_encode_machine_rw:
-    forall m,
-    decode_machine (encode_machine m) = m.
-  Axiom encode_decode_machine_rw:
-    forall w, encode_machine (decode_machine w) = w.
-  Axiom encode_machine_ext:
-    forall m1 m2,
-    encode_machine m1 = encode_machine m2 -> m1 = m2.
-
-  Axiom decode_machine_ext:
-    forall w1 w2,
-    decode_machine w1 = decode_machine w2 -> w1 = w2.
-
   (** Let us say we have a function that can encode and decode a pair of
       inputs. *)
   Parameter decode_pair : input -> (input * input).
@@ -48,11 +28,6 @@ Require Import Coq.Logic.Classical_Prop.
     forall p1 p2,
     decode_pair p1 = decode_pair p2 ->
     p1 = p2.
-
-  (** Let us define an abbreviation of the above functions. *)
-  Notation "'<<' w1 ',' w2 '>>'" := (encode_pair w1 w2).
-  Notation "'[[' M ']]'" := (encode_machine M).
-
 
   (** A language is a function that given an input (a word) holds if, and only if,
       that word is in the language. Thus, [L w] is the same as saying $w \in L$.
@@ -84,6 +59,8 @@ Require Import Coq.Logic.Classical_Prop.
   | pboth: bool -> bool -> par_result.
 
   Inductive Prog :=
+  | Read: (input -> Prog) -> Prog
+  | With: input -> Prog -> Prog
     (**
      `Seq p1 f`: run p1, if p1 terminates, then
      run (f r) where `r` is a boolean that states if p1
@@ -94,7 +71,7 @@ Require Import Coq.Logic.Classical_Prop.
       Calls a machine with a given input
       (see Universal Turing Machines)
      *)
-  | Call: machine -> input -> Prog
+  | Call: machine -> Prog
     (**
       This Turing Machine just accepts/loops/rejects without
       any further operation.
@@ -136,63 +113,72 @@ Require Import Coq.Logic.Classical_Prop.
     We can run a program `p` and obtain a resul `r` with
     `Run p r`.
     *)
-  Inductive Run: Prog -> result -> Prop :=
+  Inductive Run: Prog -> input -> result -> Prop :=
+  | run_read:
+    forall p i r,
+    Run (p i) i r ->
+    Run (Read p) i r
+  | run_with:
+    forall p i j r,
+    Run p i r ->
+    Run (With i p) j r 
   | run_ret:
     (** We can directly return a result *)
-    forall r,
-    Run (Ret r) r
+    forall r i,
+    Run (Ret r) i r
   | run_call:
     (** Calling a machine is the same as using function `run`. *)
     forall m i r,
     Exec m i r ->
-    Run (Call m i) r
+    Run (Call m) i r
   | run_seq_cont:
     (** If `p` terminates and returns `b`, then we can
        proceed with the execution of `q b`. *) 
-    forall p q b r1 r2,
-    Run p r1 ->
+    forall p q b r1 r2 i,
+    Run p i r1 ->
     Dec r1 b ->
-    Run (q b) r2 ->
-    Run (Seq p q) r2
+    Run (q b) i r2 ->
+    Run (Seq p q) i r2
   | run_seq_loop:
     (** If `p` loops, then `p; q` also loops. *)
-    forall p q,
-    Run p Loop ->
-    Run (Seq p q) Loop
+    forall p q i,
+    Run p i Loop ->
+    Run (Seq p q) i Loop
   | run_par_l_seq:
     (** If `p` terminates and `q` loops, then
        we run continuation `c` with `cleft b`. *)
-    forall p q c r1 r2 b,
-    Run p r1 ->
-    Run q Loop ->
+    forall p q c r1 r2 b i,
+    Run p i r1 ->
+    Run q i Loop ->
     Dec r1 b ->
-    Run (c (pleft b)) r2 ->
-    Run (Par p q c) r2
+    Run (c (pleft b)) i r2 ->
+    Run (Par p q c) i r2
   | run_par_r_seq:
     (** If `p` loops and `q` terminates, then
        we run continuation `c` with `cright b`. *)
-    forall p q c r1 r2 b,
-    Run p Loop ->
-    Run q r1 ->
+    forall p q c r1 r2 b i,
+    Run p i Loop ->
+    Run q i r1 ->
     Dec r1 b ->
-    Run (c (pright b)) r2 ->
-    Run (Par p q c) r2
+    Run (c (pright b)) i r2 ->
+    Run (Par p q c) i r2
   | run_par_both:
     (** If both `p` and `q` terminate, then
        we run continuation `c` with `pboth b1 b2`. *)
-    forall p1 p2 c r1 r2 r3 b1 b2,
-    Run p1 r1 ->
-    Run p2 r2 ->
+    forall p1 p2 c r1 r2 r3 b1 b2 i,
+    Run p1 i r1 ->
+    Run p2 i r2 ->
     Dec r1 b1 ->
     Dec r2 b2 ->
-    Run (c (par_choice p1 p2 b1 b2)) r3 ->
-    Run (Par p1 p2 c) r3
+    Run (c (par_choice p1 p2 b1 b2)) i r3 ->
+    Run (Par p1 p2 c) i r3
   | run_par_loop:
     (** If both `p` and `q` loop, then the whole thing loops. *)
-    forall p q c,
-    Run p Loop ->
-    Run q Loop ->
-    Run (Par p q c) Loop.
+    forall p q c i,
+    Run p i Loop ->
+    Run q i Loop ->
+    Run (Par p q c) i Loop.
+
   (** We define a notation for sequencing. *)
   Notation "'mlet' x <- e 'in' c" := (Seq e (fun x => c)) (at level 60, right associativity).
   (** We define a notion for parallel sequencing. *)
@@ -203,76 +189,96 @@ Require Import Coq.Logic.Classical_Prop.
   Notation REJECT := (Ret Reject).
   (** Notation for LOOP means returning Loop *)
   Notation LOOP := (Ret Loop).
-  (** We leave unspecified how we convert a program to a Turing machine. *)
-  Parameter Build : (input -> Prog) -> machine.
-  (** We specify the behavior of `Build` *)
-  Axiom run_build: forall p i r, Run (p i) r <-> Exec (Build p) i r.
+
+  (** We also define a function to serialize a machine into a string (of type
+      input). In the book, this corresponds to notation <M>. *)
+  Parameter encode_prog: Prog -> input.
+  (** Similarly, we have a function that takes a string and produces a machine.
+      In the book, this corresponds to notation M = <M> *)
+  Parameter decode_prog: input -> Prog.
+  (** Decoding and encoding a machine yields the same machine. *)
+  Axiom decode_encode_prog_rw:
+    forall m,
+    decode_prog (encode_prog m) = m.
+  Axiom encode_decode_prog_rw:
+    forall w, encode_prog (decode_prog w) = w.
+  Axiom encode_prog_ext:
+    forall m1 m2,
+    encode_prog m1 = encode_prog m2 -> m1 = m2.
+
+  Axiom decode_prog_ext:
+    forall w1 w2,
+    decode_prog w1 = decode_prog w2 -> w1 = w2.
 
   (** Given a machine and a string, encodes the pair as a string.
       In the book, this corresponds to notation <M, w>. *)
-  Definition encode_machine_input (M:machine) (w:input) : input :=
-    encode_pair (encode_machine M, w).
+  Definition encode_prog_input (M:Prog) (w:input) : input :=
+    encode_pair (encode_prog M, w).
 
   (** Given a string this function deserializes a pair M and w, given an encoded
       string <M,w>. *)
-  Definition decode_machine_input p := let (M, w) :=
-    decode_pair p in (decode_machine M, w).
-
-  Notation "'<[' M , w ']>'" := (encode_machine_input M w).
+  Definition decode_prog_input p := let (M, w) :=
+    decode_pair p in (decode_prog M, w).
 
   (** Decoding and encoding a pair yields the same pair. *)
-  Lemma decode_encode_machine_input_rw:
+  Lemma decode_encode_prog_input_rw:
     forall M w,
-    decode_machine_input
-          (encode_machine_input M w) = (M, w).
+    decode_prog_input
+          (encode_prog_input M w) = (M, w).
   Proof.
     intros.
-    unfold decode_machine_input.
-    unfold encode_machine_input.
+    unfold decode_prog_input.
+    unfold encode_prog_input.
     rewrite decode_encode_pair_rw.
-    rewrite decode_encode_machine_rw.
+    rewrite decode_encode_prog_rw.
     reflexivity.
   Qed.
 
-  Lemma decode_machine_input_ext:
-    forall w1 w2,
-    decode_machine_input w1 = decode_machine_input w2 ->
-    w1 = w2.
+  Lemma decode_prog_input_ext:
+    forall i1 i2,
+    decode_prog_input i1 = decode_prog_input i2 ->
+    i1 = i2.
   Proof.
-    unfold decode_machine_input.
+    unfold decode_prog_input.
     intros.
-    destruct (decode_pair w1) as (M1, i1) eqn:R1.
-    destruct (decode_pair w2) as (M2, i2) eqn:R2.
+    destruct (decode_pair i1) as (M1, j1) eqn:R1.
+    destruct (decode_pair i2) as (M2, j2) eqn:R2.
     inversion H; subst; clear H.
-    apply decode_machine_ext in H1.
+    apply decode_prog_ext in H1.
     subst.
     rewrite <- R1 in R2.
     apply decode_pair_ext in R2.
     auto.
   Qed.
 
-  Lemma decode_machine_input_rev:
+  Lemma decode_prog_input_rev:
     forall w M i,
-    decode_machine_input w = (M, i) ->
-    w = <[ M, i ]>.
+    decode_prog_input w = (M, i) ->
+    w = encode_prog_input M i.
   Proof.
     intros.
-    rewrite <- decode_encode_machine_input_rw in H.
-    apply decode_machine_input_ext in H.
+    rewrite <- decode_encode_prog_input_rw in H.
+    apply decode_prog_input_ext in H.
     assumption.
   Qed.
 
-  Lemma encode_machine_input_ext:
+  Lemma encode_prog_input_ext:
     forall M M' i i',
-    <[M, i]> = <[M', i']> -> M = M' /\ i = i'.
+    encode_prog_input M i = encode_prog_input M' i' -> M = M' /\ i = i'.
   Proof.
-    unfold encode_machine_input.
+    unfold encode_prog_input.
     intros.
     apply encode_pair_ext in H.
     inversion H; subst; clear H.
-    apply encode_machine_ext in H1.
+    apply encode_prog_ext in H1.
     auto.
   Qed.
+
+  (** Let us define an abbreviation of the above functions. *)
+  Notation "'<<' w1 ',' w2 '>>'" := (encode_pair w1 w2).
+  Notation "'[[' M ']]'" := (encode_prog M).
+  Notation "'<[' M , w ']>'" := (encode_prog_input M w).
+
 
   (** Define the equivalence of languages *)
   Definition Equiv (L1 L2:lang) :=
@@ -288,21 +294,21 @@ Require Import Coq.Logic.Classical_Prop.
   (** We use capital language to represent the recognized langauge of a machine.
       This corresponds to notation L(M). *)
 
-  Definition Lang (m:machine) : lang := fun i => Exec m i Accept.
+  Definition Lang (p:Prog) : lang := fun i => Run p i Accept.
 
   (** We use a direct definition of recognition:
       The turing machine accepts input i (with `run m i`)
       iff language L accepts i.
        *)
 
-  Definition Recognizes (m:machine) (L:lang) :=
-    forall i, Exec m i Accept <-> L i.
+  Definition Recognizes (p:Prog) (L:lang) :=
+    forall i, Run p i Accept <-> L i.
 
   Lemma recognizes_def:
-    forall m (L:lang),
-    (forall i, Exec m i Accept -> L i) ->
-    (forall i, L i -> Exec m i Accept) ->
-    Recognizes m L.
+    forall p (L:lang),
+    (forall i, Run p i Accept -> L i) ->
+    (forall i, L i -> Run p i Accept) ->
+    Recognizes p L.
   Proof.
     intros.
     unfold Recognizes.
@@ -410,7 +416,8 @@ Require Import Coq.Logic.Classical_Prop.
   (** A language is recognizable, that is
       there is some machine m that recognizes it. *)
 
-  Definition Recognizable (L:lang) : Prop := exists m, Recognizes m L.
+  Definition Recognizable (L:lang) : Prop :=
+    exists m, Recognizes m L.
 
   Global Instance recognizable_equiv_proper: Proper (Equiv ==> iff) Recognizable.
   Proof.
@@ -469,24 +476,133 @@ Require Import Coq.Logic.Classical_Prop.
       - contradiction.
     Qed.
 
+
+    Ltac clear_dec :=
+      match goal with
+        | [ H1: Dec ?r ?b1, H2: Dec ?r ?b2 |- _] =>
+          assert (Hx: b1 = b2) by eauto using dec_fun;
+          rewrite Hx in *;
+          clear H2 Hx
+        | [ H: Dec Loop _ |- _ ] => inversion H
+        end.
+
+    Lemma run_fun:
+      forall p i r1,
+      Run p i r1 ->
+      forall r2,
+      Run p i r2 ->
+      r1 = r2.
+    Proof.
+      intros p i r1 H; induction H; intros r' He;
+        inversion He; subst; clear He; auto;
+        (* In each case we have a bunch of Run's that are solved
+           by induction; we need to make sure we clear any dec's,
+           so that we can advance to the next IH *)
+        repeat match goal with
+        | [ H1: Run ?q i ?r1, H2: Run ?q i ?r2 |- _] =>
+          (
+            assert (r1 = r2) by eauto ||
+            assert (r2 = r1) by eauto
+          ); subst; clear H2; try clear_dec; auto
+        end;
+        try clear_dec; auto.
+      eauto using exec_fun.
+    Qed.
+
+    Lemma run_exists:
+      forall p i,
+      exists r, Run p i r.
+    Proof.
+      induction p; intros.
+      - assert (H := H i i).
+        destruct H as (r, Hr).
+        exists r.
+        constructor; auto.
+      - assert (IHp := IHp i).
+        destruct IHp as (r, IHp).
+        exists r.
+        constructor.
+        assumption.
+      - assert (IHp := IHp i).
+        destruct IHp as ([], IHp).
+        + assert (H := H true i).
+          destruct H as (r, H).
+          exists r.
+          eapply run_seq_cont; eauto.
+          constructor.
+        + assert (H := H false i).
+          destruct H as (r, H).
+          exists r.
+          eapply run_seq_cont; eauto.
+          constructor.
+        + exists Loop.
+          constructor.
+          assumption.
+      - destruct (exec_exists m i) as (r, He).
+        exists r.
+        constructor.
+        assumption.
+      - exists r.
+        constructor.
+      - assert (IHp1 := IHp1 i).
+        assert (IHp2 := IHp2 i).
+        destruct IHp1 as (r1, Hr1).
+        destruct IHp2 as (r2, Hr2).
+        destruct r1, r2.
+        + assert (H := H (par_choice p1 p2 true true) i).
+          destruct H as (r, Hr).
+          exists r.
+          eapply run_par_both; eauto using dec_accept.
+        + assert (H := H (par_choice p1 p2 true false) i).
+          destruct H as (r, Hr).
+          exists r.
+          eapply run_par_both; eauto using dec_accept, dec_reject.
+        + assert (H := H (pleft true) i).
+          destruct H as (r, Hr).
+          exists r.
+          eapply run_par_l_seq; eauto; constructor.
+        + assert (H := H (par_choice p1 p2 false true) i).
+          destruct H as (r, Hr).
+          exists r.
+          eapply run_par_both; eauto using dec_accept, dec_reject.
+        + assert (H := H (par_choice p1 p2 false false) i).
+          destruct H as (r, Hr).
+          exists r.
+          eapply run_par_both; eauto using dec_accept, dec_reject.
+        + assert (H := H (pleft false) i).
+          destruct H as (r, Hr).
+          exists r.
+          eapply run_par_l_seq; eauto; constructor.
+        + assert (H := H (pright true) i).
+          destruct H as (r, Hr).
+          exists r.
+          eapply run_par_r_seq; eauto; constructor.
+        + assert (H := H (pright false) i).
+          destruct H as (r, Hr).
+          exists r.
+          eapply run_par_r_seq; eauto; constructor.
+        + exists Loop.
+          constructor; auto.
+    Qed.
+
     Lemma recognizes_run_reject:
-      forall m L i,
-      Recognizes m L ->
-      Exec m i Reject ->
+      forall p L i,
+      Recognizes p L ->
+      Run p i Reject ->
       ~ L i.
     Proof.
       intros.
       intros N.
       apply H in N.
-      assert (Hx: Reject = Accept) by eauto using exec_fun.
+      assert (Hx: Reject = Accept) by eauto using run_fun.
       inversion Hx.
     Qed.
 
     Lemma recognizes_run_accept:
-      forall m L,
-      Recognizes m L ->
+      forall p L,
+      Recognizes p L ->
       forall i,
-      Exec m i Accept ->
+      Run p i Accept ->
       L i.
     Proof.
       intros.
@@ -496,25 +612,22 @@ Require Import Coq.Logic.Classical_Prop.
 
 
     Lemma recognizes_not_accept:
-      forall m L i,
-      Recognizes m L ->
+      forall p L i,
+      Recognizes p L ->
       ~ L i ->
-      forall r,
-      Exec m i r ->
-      r <> Accept.
+      ~ Run p i Accept.
     Proof.
       intros.
       intros N.
-      subst.
       assert (L i). { eapply recognizes_run_accept; eauto. }
       contradiction.
     Qed.
 
     Lemma recognizes_accept:
-      forall m L i,
-      Recognizes m L ->
+      forall p L i,
+      Recognizes p L ->
       L i ->
-      Exec m i Accept.
+      Run p i Accept.
     Proof.
       intros.
       apply H in H0.
@@ -522,16 +635,16 @@ Require Import Coq.Logic.Classical_Prop.
     Qed.
 
     Lemma recognizes_run_loop:
-      forall m L,
-      Recognizes m L ->
+      forall p L,
+      Recognizes p L ->
       forall i,
-      Exec m i Loop ->
+      Run p i Loop ->
       ~ L i.
     Proof.
       intros.
       intros N.
       apply H in N.
-      assert (Hx: Loop = Accept) by eauto using exec_fun.
+      assert (Hx: Loop = Accept) by eauto using run_fun.
       inversion Hx.
     Qed.
 
@@ -576,7 +689,7 @@ Require Import Coq.Logic.Classical_Prop.
     Lemma co_recognizes_run_accept:
       forall m L i,
       Recognizes m (compl L) ->
-      Exec m i Accept ->
+      Run m i Accept ->
       ~ L i.
     Proof.
       intros.
@@ -587,14 +700,11 @@ Require Import Coq.Logic.Classical_Prop.
       forall m L i,
       Recognizes m (compl L) ->
       L i ->
-      forall r,
-      Exec m i r -> 
-      r <> Accept.
+      ~ Run m i Accept.
     Proof.
       intros.
       intros N.
-      subst.
-      apply H in H1.
+      apply H in N.
       contradiction.
     Qed.
 
@@ -602,7 +712,7 @@ Require Import Coq.Logic.Classical_Prop.
       forall m L i,
       Recognizes m (compl L) ->
       ~ L i ->
-      Exec m i Accept.
+      Run m i Accept.
     Proof.
       intros.
       unfold compl in *.
@@ -617,11 +727,11 @@ Require Import Coq.Logic.Classical_Prop.
   Section Decidable.
     (** We define a decider as any Turing Machine that returns either Accept or
         Reject, but not Loop. *)
-    Definition Decider d := forall i r, Exec d i r -> r <> Loop.
+    Definition Decider (d:Prog) := forall i, ~ Run d i Loop.
 
     Lemma decider_def:
       forall d,
-      (forall i r, Exec d i r -> r <> Loop) ->
+      (forall i, ~ Run d i Loop) ->
       Decider d.
     Proof.
       intros.
@@ -687,30 +797,30 @@ Require Import Coq.Logic.Classical_Prop.
     Lemma decides_run_reject:
       forall m L i,
       Decides m L ->
-      Exec m i Reject ->
+      Run m i Reject ->
       ~ L i.
     Proof.
       intros.
       apply decides_to_recognizes in H.
-      apply recognizes_run_reject with (m:=m); auto.
+      apply recognizes_run_reject with (p:=m); auto.
     Qed.
 
     Lemma decides_run_accept:
       forall m L i,
       Decides m L ->
-      Exec m i Accept ->
+      Run m i Accept ->
       L i.
     Proof.
       intros.
       apply decides_to_recognizes in H.
-      apply recognizes_run_accept with (m:=m); auto.
+      apply recognizes_run_accept with (p:=m); auto.
     Qed.
 
     Lemma decides_accept:
       forall m L i,
       Decides m L ->
       L i ->
-      Exec m i Accept.
+      Run m i Accept.
     Proof.
       intros.
       apply decides_to_recognizes in H.
@@ -721,27 +831,26 @@ Require Import Coq.Logic.Classical_Prop.
       forall m,
       Decider m ->
       forall i,
-      Exec m i Accept \/ Exec m i Reject.
+      Run m i Accept \/ Run m i Reject.
     Proof.
       intros.
       unfold Decider in *.
       assert (H:=H i).
-      destruct (exec_exists m i) as (r, He);  auto.
-      assert (r <> Loop) by auto.
+      destruct (run_exists m i) as (r, He);  auto.
       destruct r; auto.
       contradiction.
     Qed.
 
     Lemma decider_to_dec:
-      forall m w r,
+      forall m i r,
       Decider m ->
-      Exec m w r ->
+      Run m i r ->
       exists b, Dec r b.
     Proof.
       intros.
-      apply decider_to_run with (i:=w) in H.
+      apply decider_to_run with (i:=i) in H.
       assert (Hx: r = Accept \/ r = Reject). {
-        intuition; eauto using exec_fun.
+        intuition; eauto using run_fun.
       }
       destruct Hx;subst.
       - exists true.
@@ -753,11 +862,11 @@ Require Import Coq.Logic.Classical_Prop.
     Lemma decider_to_p_run:
       forall m,
       Decider m ->
-      forall w,
-      exists r b, Run (Call m w) r /\ Dec r b.
+      forall i,
+      exists r b, Run m i r /\ Dec r b.
     Proof.
       intros.
-      destruct (exec_exists m w) as (r, He).
+      destruct (run_exists m i) as (r, He).
       exists r.
       assert (Hx : exists b, Dec r b) by eauto using decider_to_dec.
       destruct Hx as (b, Hx).
@@ -778,7 +887,7 @@ Require Import Coq.Logic.Classical_Prop.
       forall m L i,
       Decides m L ->
       ~ L i ->
-      Exec m i Reject.
+      Run m i Reject.
     Proof.
       intros.
       destruct H.
@@ -790,25 +899,20 @@ Require Import Coq.Logic.Classical_Prop.
     Qed.
 
     Lemma decider_no_loop:
-      forall m i r,
+      forall m i,
       Decider m ->
-      Exec m i r ->
-      r <> Loop.
+      ~ Run m i Loop.
     Proof.
       intros.
-      intros N.
-      subst.
       unfold Decider in *.
-      apply H in H0.
-      contradiction.
+      auto.
     Qed.
 
     Lemma decides_no_loop:
-      forall m L i,
+      forall m L,
       Decides m L ->
-      forall r,
-      Exec m i r ->
-      r <> Loop.
+      forall i,
+      ~ Run m i Loop.
     Proof.
       intros.
       destruct H.
@@ -818,70 +922,21 @@ Require Import Coq.Logic.Classical_Prop.
     Lemma decider_not_reject_to_accept:
       forall d i,
       Decider d ->
-      forall r,
-      Exec d i r ->
-      r <> Reject ->
-      r = Accept.
+      ~ Run d i Reject ->
+      Run d i Accept.
     Proof.
       intros.
-      apply decider_no_loop in H0; auto.
-      destruct r; auto; contradiction.
-    Qed.
-  (*
-    Definition Predicate M f :=
-      (forall w, Exec M w Accept <-> f w = true) /\
-      (forall w, Exec M w Reject <-> f w = false). 
-
-    Lemma decider_to_predicate:
-      forall M L,
-      Decides M L ->
-      exists f, Predicate M f.
-    Proof.
-      intros.
-      exists (fun w =>
-        match run M w with
-        | Accept => true
-        | _ => false
-        end).
-      unfold Predicate.
-      split; split; intros.
-      - rewrite H0.
-        reflexivity.
-      - destruct (run M w); auto; inversion H0.
-      - rewrite H0.
-        reflexivity.
-      - destruct (run M w) eqn:Hr; auto; inversion H0.
-        apply H in Hr.
-        contradiction.
+      apply decider_no_loop with (i:=i) in H; eauto.
+      destruct (run_exists d i) as ([], He); auto; contradiction.
     Qed.
 
-    Lemma predicate_accept:
-      forall M f w,
-      Predicate M f ->
-      run M w = Accept <-> f w = true.
-    Proof.
-      intros.
-      destruct H as (H1, H2).
-      auto.
-    Qed.
-
-    Lemma predicate_reject:
-      forall M f w,
-      Predicate M f ->
-      run M w = Reject <-> f w = false.
-    Proof.
-      intros.
-      destruct H as (H1, H2).
-      auto.
-    Qed.
-*)
   End Decidable.
 
   Definition halt_with (b:bool) := Ret (if b then Accept else Reject).
 
   Definition Empty : lang := fun p => False.
   Definition IsEmpty M := Recognizes M Empty.
-  Definition NeverAccept M := (forall w r, Exec M w r -> r <> Accept).
+  Definition NeverAccept M := (forall (i:input), ~ Run M i Accept).
 
   Section RUN.
 
@@ -889,41 +944,39 @@ Require Import Coq.Logic.Classical_Prop.
       forall m L i,
       Recognizes m L ->
       L i ->
-      Run (Call m i) Accept.
+      Run m i Accept.
     Proof.
       intros.
-      apply run_call.
-      apply recognizes_accept with (m:=m) in H0; auto.
+      apply H; assumption.
     Qed.
 
     Lemma run_call_decides_accept:
       forall m L i,
       Decides m L ->
       L i ->
-      Run (Call m i) Accept.
+      Run m i Accept.
     Proof.
       intros.
-      apply run_call.
-      apply decides_accept with (m:=m) in H0; auto.
+      apply H.
+      assumption.
     Qed.
 
     Lemma run_call_decides_reject:
       forall m L i,
       Decides m L ->
       ~ L i ->
-      Run (Call m i) Reject.
+      Run m i Reject.
     Proof.
       intros.
-      apply run_call.
-      apply decides_reject with (m:=m) in H0; auto.
+      eapply decides_reject; eauto.
     Qed.
 
     Lemma run_par_l_accept:
-      forall p q c r,
-      Run p Accept ->
-      Run q Loop ->
-      Run (c (pleft true)) r ->
-      Run (Par p q c) r.
+      forall i p q c r,
+      Run p i Accept ->
+      Run q i Loop ->
+      Run (c (pleft true)) i r ->
+      Run (Par p q c) i r.
     Proof.
       intros.
       apply run_par_l_seq with (r1:=Accept) (b:=true); auto.
@@ -931,11 +984,11 @@ Require Import Coq.Logic.Classical_Prop.
     Qed.
 
     Lemma run_par_r_accept:
-      forall p q c r,
-      Run q Accept ->
-      Run p Loop ->
-      Run (c (pright true)) r ->
-      Run (Par p q c) r.
+      forall i p q c r,
+      Run q i Accept ->
+      Run p i Loop ->
+      Run (c (pright true)) i r ->
+      Run (Par p q c) i r.
     Proof.
       intros.
       apply run_par_r_seq with (r1:=Accept) (b:=true); auto.
@@ -943,11 +996,11 @@ Require Import Coq.Logic.Classical_Prop.
     Qed.
 
     Lemma run_par_l_reject:
-      forall p q c r,
-      Run p Reject ->
-      Run q Loop ->
-      Run (c (pleft false)) r ->
-      Run (Par p q c) r.
+      forall i p q c r,
+      Run p i Reject ->
+      Run q i Loop ->
+      Run (c (pleft false)) i r ->
+      Run (Par p q c) i r.
     Proof.
       intros.
       apply run_par_l_seq with (r1:=Reject) (b:=false); auto.
@@ -955,11 +1008,11 @@ Require Import Coq.Logic.Classical_Prop.
     Qed.
 
     Lemma run_par_r_reject:
-      forall p q c r,
-      Run p Loop ->
-      Run q Reject ->
-      Run (c (pright false)) r ->
-      Run (Par p q c) r.
+      forall i p q c r,
+      Run p i Loop ->
+      Run q i Reject ->
+      Run (c (pright false)) i r ->
+      Run (Par p q c) i r.
     Proof.
       intros.
       apply run_par_r_seq with (r1:=Reject) (b:=false); auto.
@@ -967,10 +1020,10 @@ Require Import Coq.Logic.Classical_Prop.
     Qed.
 
     Lemma run_seq_reject:
-      forall p q r,
-      Run p Reject ->
-      Run (q false) r ->
-      Run (Seq p q) r.
+      forall i p q r,
+      Run p i Reject ->
+      Run (q false) i r ->
+      Run (Seq p q) i r.
     Proof.
       intros.
       apply run_seq_cont with (b:=false) (r1:=Reject).
@@ -980,10 +1033,10 @@ Require Import Coq.Logic.Classical_Prop.
     Qed.
 
     Lemma run_seq_accept:
-      forall p q r,
-      Run p Accept ->
-      Run (q true) r ->
-      Run (Seq p q) r.
+      forall i p q r,
+      Run p i Accept ->
+      Run (q true) i r ->
+      Run (Seq p q) i r.
     Proof.
       intros.
       apply run_seq_cont with (b:=true) (r1:=Accept).
@@ -993,11 +1046,11 @@ Require Import Coq.Logic.Classical_Prop.
     Qed.
 
     Lemma run_par_accept_reject:
-      forall p q c r,
-      Run p Accept ->
-      Run q Reject ->
-      Run (c (par_choice p q true false)) r ->
-      Run (Par p q c) r.
+      forall i p q c r,
+      Run p i Accept ->
+      Run q i Reject ->
+      Run (c (par_choice p q true false)) i r ->
+      Run (Par p q c) i r.
     Proof.
       intros.
       apply run_par_both with (r1:=Accept) (r2:=Reject) (b1:=true) (b2:=false);
@@ -1005,8 +1058,8 @@ Require Import Coq.Logic.Classical_Prop.
     Qed.
 
     Lemma run_halt_with_to_dec:
-      forall b r,
-      Run (halt_with b) r ->
+      forall i b r,
+      Run (halt_with b) i r ->
       Dec r b.
     Proof.
       intros.
@@ -1017,8 +1070,8 @@ Require Import Coq.Logic.Classical_Prop.
     Qed.
 
     Lemma run_halt_with_inv_accept:
-      forall b,
-      Run (halt_with b) Accept ->
+      forall i b,
+      Run (halt_with b) i Accept ->
       b = true.
     Proof.
       intros.
@@ -1028,8 +1081,8 @@ Require Import Coq.Logic.Classical_Prop.
     Qed.
 
     Lemma run_halt_with_inv_reject:
-      forall b,
-      Run (halt_with b) Reject ->
+      forall i b,
+      Run (halt_with b) i Reject ->
       b = false.
     Proof.
       intros.
@@ -1039,47 +1092,17 @@ Require Import Coq.Logic.Classical_Prop.
     Qed.
 
     Lemma run_halt_with_true:
-      Run (halt_with true) Accept.
+      forall i,
+      Run (halt_with true) i Accept.
     Proof.
       apply run_ret.
     Qed.
 
     Lemma run_halt_with_false:
-      Run (halt_with false) Reject.
+      forall i,
+      Run (halt_with false) i Reject.
     Proof.
       apply run_ret.
-    Qed.
-
-    Ltac clear_dec :=
-      match goal with
-        | [ H1: Dec ?r ?b1, H2: Dec ?r ?b2 |- _] =>
-          assert (Hx: b1 = b2) by eauto using dec_fun;
-          rewrite Hx in *;
-          clear H2 Hx
-        | [ H: Dec Loop _ |- _ ] => inversion H
-        end.
-
-    Lemma run_fun:
-      forall p r1,
-      Run p r1 ->
-      forall r2,
-      Run p r2 ->
-      r1 = r2.
-    Proof.
-      intros p r1 H; induction H; intros r' He;
-        inversion He; subst; clear He; auto;
-        (* In each case we have a bunch of Run's that are solved
-           by induction; we need to make sure we clear any dec's,
-           so that we can advance to the next IH *)
-        repeat match goal with
-        | [ H1: Run ?q ?r1, H2: Run ?q ?r2 |- _] =>
-          (
-            assert (r1 = r2) by eauto ||
-            assert (r2 = r1) by eauto
-          ); subst; clear H2; try clear_dec; auto
-        end;
-        try clear_dec; auto.
-      eauto using exec_fun.
     Qed.
 
   End RUN.
@@ -1090,11 +1113,11 @@ Require Import Coq.Logic.Classical_Prop.
     programs.
     *)
   Section P_DECIDER.
-    Definition PAccepts (p:input->Prog) i := Run (p i) Accept.
+    Definition PAccepts (p:Prog) i := Run p i Accept.
 
     Lemma p_accepts_def:
       forall p i,
-      Run (p i) Accept ->
+      Run p i Accept ->
       PAccepts p i.
     Proof.
       intros.
@@ -1102,22 +1125,24 @@ Require Import Coq.Logic.Classical_Prop.
     Qed.
 
     (* A program halts *)
-    Definition PHalts p := exists r, Run p r /\ r <> Loop.
+    Definition PHalts p i := ~ Run p i Loop.
 
     Lemma p_halts_def:
-      forall r p,
-      Run p r ->
+      forall i r p,
+      Run p i r ->
       r <> Loop ->
-      PHalts p.
+      PHalts p i.
     Proof.
       unfold PHalts; intros.
-      eauto.
+      intros N.
+      assert (r = Loop) by eauto using run_fun.
+      contradiction.
     Qed.
 
     Lemma p_halts_accept:
-      forall p,
-      Run p Accept ->
-      PHalts p.
+      forall p i,
+      Run p i Accept ->
+      PHalts p i.
     Proof.
       intros.
       apply p_halts_def with (r:=Accept).
@@ -1126,9 +1151,9 @@ Require Import Coq.Logic.Classical_Prop.
     Qed.
 
     Lemma p_halts_reject:
-      forall p,
-      Run p Reject ->
-      PHalts p.
+      forall p i,
+      Run p i Reject ->
+      PHalts p i.
     Proof.
       intros.
       apply p_halts_def with (r:=Reject).
@@ -1137,37 +1162,41 @@ Require Import Coq.Logic.Classical_Prop.
     Qed.
 
     Lemma p_halts_loop:
-      forall p,
-      Run p Loop ->
-      ~ PHalts p.
+      forall p i,
+      Run p i Loop ->
+      ~ PHalts p i.
     Proof.
       intros.
       intros N.
-      destruct N as (r, (Hr, ?)).
-      assert (r = Loop) by eauto using run_fun.
-      contradiction.
+      apply N in H.
+      assumption.
     Qed.
 
     Lemma p_halts_ret_accept:
-      PHalts (Ret Accept).
+      forall i,
+      PHalts (Ret Accept) i.
     Proof.
-      apply p_halts_def with (r:=Accept).
-      - apply run_ret.
-      - intros N; inversion N.
+      intros.
+      unfold PHalts.
+      intros N.
+      inversion N.
     Qed.
 
     Lemma p_halts_ret_reject:
-      PHalts (Ret Reject).
+      forall i,
+      PHalts (Ret Reject) i.
     Proof.
-      apply p_halts_def with (r:=Reject).
-      - apply run_ret.
-      - intros N; inversion N.
+      intros.
+      unfold PHalts.
+      intros N.
+      inversion N.
     Qed.
 
     Lemma p_halts_dec:
       forall r b,
       Dec r b ->
-      PHalts (Ret r).
+      forall i,
+      PHalts (Ret r) i.
     Proof.
       intros.
       apply p_halts_def with (r:=r).
@@ -1177,17 +1206,23 @@ Require Import Coq.Logic.Classical_Prop.
     Qed.
 
     Lemma p_halts_seq:
-      forall p q r b,
-      Run p r ->
+      forall i p q r b,
+      Run p i r ->
       Dec r b ->
-      PHalts (q b) ->
-      PHalts (Seq p q).
+      PHalts (q b) i ->
+      PHalts (Seq p q) i.
     Proof.
       intros.
-      destruct H1 as (r1, (H1, H2)).
-      apply p_halts_def with (r:=r1).
-      - apply run_seq_cont with (b:=b) (r1:=r); auto.
-      - assumption.
+      intros N.
+      inversion N; subst; clear N.
+      + assert (r1 = r) by eauto using run_fun.
+        subst.
+        assert (b0 = b) by eauto using dec_fun.
+        subst.
+        apply H1; auto.
+      + assert (r = Loop) by eauto using run_fun.
+        subst.
+        inversion H0.
     Qed.
 
     Inductive ParMerge p q : result -> result -> par_result -> Prop :=
@@ -1253,186 +1288,215 @@ Require Import Coq.Logic.Classical_Prop.
       auto using par_merge_right, dec_accept, dec_reject.
     Qed.
 
-    Lemma run_exists_any:
-      forall (p:input->Prog) i, exists r, Run (p i) r.
+    Lemma p_halts_inv:
+      forall p i,
+      PHalts p i ->
+      Run p i Accept \/ Run p i Reject.
     Proof.
       intros.
-      destruct (exec_exists (Build p) i) as (r, He).
-      exists r.
-      apply run_build.
-      assumption.
+      unfold PHalts in *.
+      destruct (run_exists p i) as (r, Hr).
+      destruct r; auto.
+      contradiction.
     Qed.
 
-    Lemma run_exists:
-      forall p,
-      exists r, Run p r.
+    Lemma p_halts_par_both:
+      forall k p1 p2 b1 b2 r1 r2 i,
+      Run p1 i r1 ->
+      Run p2 i r2 ->
+      Dec r1 b1 ->
+      Dec r2 b2 ->
+      PHalts (k (par_choice p1 p2 b1 b2)) i ->
+      PHalts (Par p1 p2 k) i.
     Proof.
       intros.
-      destruct (run_exists_any (fun x=>p) input_inhabited) as (r, H).
-      eauto.
+      apply p_halts_inv in H3.
+      intuition.
+      - apply p_halts_accept.
+        eapply run_par_both; eauto.
+      - apply p_halts_reject.
+        eapply run_par_both; eauto.
+    Qed.
+
+    Lemma p_halts_par_l_seq:
+      forall k p1 p2 b r i,
+      Run p1 i r ->
+      Run p2 i Loop ->
+      Dec r b ->
+      PHalts (k (pleft b)) i ->
+      PHalts (Par p1 p2 k) i.
+    Proof.
+      intros.
+      apply p_halts_inv in H2.
+      intuition.
+      - apply p_halts_accept.
+        eapply run_par_l_seq; eauto.
+      - apply p_halts_reject.
+        eapply run_par_l_seq; eauto.
+    Qed.
+
+    Lemma p_halts_par_r_seq:
+      forall k p1 p2 b r i,
+      Run p1 i Loop ->
+      Run p2 i r ->
+      Dec r b ->
+      PHalts (k (pright b)) i ->
+      PHalts (Par p1 p2 k) i.
+    Proof.
+      intros.
+      apply p_halts_inv in H2.
+      intuition.
+      - apply p_halts_accept.
+        eapply run_par_r_seq; eauto.
+      - apply p_halts_reject.
+        eapply run_par_r_seq; eauto.
     Qed.
 
     Lemma p_halts_par_l:
-      forall r1 b p1 p2 k,
-      Run p1 r1 ->
+      forall i r1 b p1 p2 k,
+      Run p1 i r1 ->
       Dec r1 b ->
-      (forall r2 q, Run p2 r2 -> ParMerge p1 p2 r1 r2 q -> PHalts (k q)) ->
-      PHalts (Par p1 p2 k).
+      (forall r2 q, Run p2 i r2 -> ParMerge p1 p2 r1 r2 q -> PHalts (k q) i) ->
+      PHalts (Par p1 p2 k) i.
     Proof.
       intros.
       inversion H0; subst; clear H0.
-      - destruct (run_exists p2) as (r2, Hp2).
+      - destruct (run_exists p2 i) as (r2, Hp2).
+        intros N.
         destruct r2.
-        + assert (PHalts (k (par_choice p1 p2 true true))). {
+        + assert (Hp: PHalts (k (par_choice p1 p2 true true)) i). {
             apply H1 with (r2:=Accept); auto.
             apply par_merge_accept_accept.
           }
-          destruct H0 as (r, (Hr,?)).
-          apply p_halts_def with (r:=r); auto.
-          eapply run_par_both; eauto using dec_accept.
-        + assert (PHalts (k (par_choice p1 p2 true false))). {
+          eapply p_halts_par_both in Hp; eauto using dec_accept.
+        + assert (Hp: PHalts (k (par_choice p1 p2 true false)) i). {
             apply H1 with (r2:=Reject); auto.
             apply par_merge_accept_reject.
           }
-          destruct H0 as (r, (Hr,?)).
-          apply p_halts_def with (r:=r); auto.
-          eapply run_par_both; eauto using dec_reject, dec_accept.
-        + assert (PHalts (k (pleft true))). {
+          eapply p_halts_par_both in Hp; eauto using dec_accept, dec_reject.
+        + assert (Hp: PHalts (k (pleft true)) i). {
             apply H1 with (r2:=Loop); auto.
             apply par_merge_accept_loop.
           }
-          destruct H0 as (r, (Hr,?)).
-          apply p_halts_def with (r:=r); auto.
-          eapply run_par_l_seq; eauto using dec_accept.
-      - destruct (run_exists p2) as (r2, Hp2).
+          eapply p_halts_par_l_seq in Hp; eauto using dec_accept.
+      - destruct (run_exists p2 i) as (r2, Hp2).
         destruct r2.
-        + assert (PHalts (k (par_choice p1 p2 false true))). {
+        + assert (Hp: PHalts (k (par_choice p1 p2 false true)) i). {
             apply H1 with (r2:=Accept); auto.
             apply par_merge_reject_accept.
           }
-          destruct H0 as (r, (Hr,?)).
-          apply p_halts_def with (r:=r); auto.
-          eapply run_par_both; eauto using dec_accept, dec_reject.
-        + assert (PHalts (k (par_choice p1 p2 false false))). {
+          eapply p_halts_par_both in Hp; eauto using dec_accept, dec_reject.
+        + assert (Hp: PHalts (k (par_choice p1 p2 false false)) i). {
             apply H1 with (r2:=Reject); auto.
             apply par_merge_reject_reject.
           }
-          destruct H0 as (r, (Hr,?)).
-          apply p_halts_def with (r:=r); auto.
-          eapply run_par_both; eauto using dec_reject, dec_accept.
-        + assert (PHalts (k (pleft false))). {
+          eapply p_halts_par_both in Hp; eauto using dec_accept, dec_reject.
+        + assert (Hp: PHalts (k (pleft false)) i). {
             apply H1 with (r2:=Loop); auto.
             apply par_merge_reject_loop.
           }
-          destruct H0 as (r, (Hr,?)).
-          apply p_halts_def with (r:=r); auto.
-          eapply run_par_l_seq; eauto using dec_accept, dec_reject.
+          eapply p_halts_par_l_seq in Hp; eauto using dec_accept, dec_reject.
     Qed.
 
     Lemma p_halts_par_r:
-      forall r2 b p1 p2 k,
-      Run p2 r2 ->
+      forall i r2 b p1 p2 k,
+      Run p2 i r2 ->
       Dec r2 b ->
-      (forall r1 q, Run p1 r1 -> ParMerge p1 p2 r1 r2 q -> PHalts (k q)) ->
-      PHalts (Par p1 p2 k).
+      (forall r1 q, Run p1 i r1 -> ParMerge p1 p2 r1 r2 q -> PHalts (k q) i) ->
+      PHalts (Par p1 p2 k) i.
     Proof.
       intros.
       inversion H0; subst; clear H0.
-      - destruct (run_exists p1) as (r1, Hp1).
+      - destruct (run_exists p1 i) as (r1, Hp1).
         destruct r1.
-        + assert (PHalts (k (par_choice p1 p2 true true))). {
+        + assert (Hp: PHalts (k (par_choice p1 p2 true true)) i). {
             apply H1 with (r1:=Accept); auto.
             apply par_merge_accept_accept.
           }
-          destruct H0 as (r, (Hr,?)).
-          apply p_halts_def with (r:=r); auto.
-          eapply run_par_both; eauto using dec_accept.
-        + assert (PHalts (k (par_choice p1 p2 false true))). {
+          eapply p_halts_par_both in Hp; eauto using dec_accept, dec_reject.
+        + assert (Hp: PHalts (k (par_choice p1 p2 false true)) i). {
             apply H1 with (r1:=Reject); auto.
             apply par_merge_reject_accept.
           }
-          destruct H0 as (r, (Hr,?)).
-          apply p_halts_def with (r:=r); auto.
-          eapply run_par_both; eauto using dec_reject, dec_accept.
-        + assert (PHalts (k (pright true))). {
+          eapply p_halts_par_both in Hp; eauto using dec_accept, dec_reject.
+        + assert (Hp: PHalts (k (pright true)) i). {
             apply H1 with (r1:=Loop); auto.
             apply par_merge_loop_accept.
           }
-          destruct H0 as (r, (Hr,?)).
-          apply p_halts_def with (r:=r); auto.
-          eapply run_par_r_seq; eauto using dec_accept.
-      - destruct (run_exists p1) as (r1, Hp1).
+          eapply p_halts_par_r_seq in Hp; eauto using dec_accept.
+      - destruct (run_exists p1 i) as (r1, Hp1).
         destruct r1.
-        + assert (PHalts (k (par_choice p1 p2 true false))). {
+        + assert (Hp: PHalts (k (par_choice p1 p2 true false)) i). {
             apply H1 with (r1:=Accept); auto.
             apply par_merge_accept_reject.
           }
-          destruct H0 as (r, (Hr,?)).
-          apply p_halts_def with (r:=r); auto.
-          eapply run_par_both; eauto using dec_accept, dec_reject.
-        + assert (PHalts (k (par_choice p1 p2 false false))). {
+          eapply p_halts_par_both in Hp; eauto using dec_accept, dec_reject.
+        + assert (Hp: PHalts (k (par_choice p1 p2 false false)) i). {
             apply H1 with (r1:=Reject); auto.
             apply par_merge_reject_reject.
           }
-          destruct H0 as (r, (Hr,?)).
-          apply p_halts_def with (r:=r); auto.
-          eapply run_par_both; eauto using dec_reject, dec_accept.
-        + assert (PHalts (k (pright false))). {
+          eapply p_halts_par_both in Hp; eauto using dec_accept, dec_reject.
+        + assert (Hp: PHalts (k (pright false)) i). {
             apply H1 with (r1:=Loop); auto.
             apply par_merge_loop_reject.
           }
-          destruct H0 as (r, (Hr,?)).
-          apply p_halts_def with (r:=r); auto.
-          eapply run_par_r_seq; eauto using dec_accept, dec_reject.
+          eapply p_halts_par_r_seq in Hp; eauto using dec_accept, dec_reject.
     Qed.
 
     Lemma p_halts_call:
-      forall m w r,
-      Exec m w r ->
-      r <> Loop ->
-      PHalts (Call m w).
+      forall m i,
+      ~ Exec m i Loop ->
+      PHalts (Call m) i.
     Proof.
-      eauto using p_halts_def, run_call.
+      intros.
+      destruct (exec_exists m i) as (r, He).
+      apply p_halts_def with (r:=r); eauto using run_call.
+      intros N.
+      subst.
+      contradiction.
     Qed.
 
     Lemma p_halts_call_decider:
       forall m i,
       Decider m ->
-      PHalts (Call m i).
+      PHalts m i.
     Proof.
       intros.
       assert (H := H i).
-      destruct (exec_exists m i) as (r, He).
-      eauto using p_halts_call.
+      destruct (run_exists m i) as (r, He).
+      eapply p_halts_def; eauto.
+      intros N.
+      subst.
+      contradiction.
     Qed.
 
     Lemma p_halts_seq_call:
-      forall m w r k b,
-      Exec m w r ->
+      forall m i r k b,
+      Exec m i r ->
       Dec r b ->
-      PHalts (k b) ->
-      PHalts (Seq (Call m w) k).
+      PHalts (k b) i ->
+      PHalts (Seq (Call m) k) i.
     Proof.
       intros.
       apply p_halts_seq with (r:=r) (b:=b); auto using run_call.
     Qed.
 
     Lemma p_halts_seq_call_decider:
-      forall m w k,
+      forall m i k,
       Decider m ->
-      (forall r b, Run (Call m w) r -> Dec r b -> PHalts (k b)) ->
-      PHalts (Seq (Call m w) k).
+      (forall r b, Run m i r -> Dec r b -> PHalts (k b) i) ->
+      PHalts (Seq m k) i.
     Proof.
       intros.
-      apply decider_to_p_run with (w:=w) in H.
-      destruct H as (r, (b, (Hr, Hd))).
+      destruct decider_to_p_run with (m:=m) (i:=i)
+       as (r, (b, (Ha, Hb))); auto.
       apply p_halts_seq with (r:=r) (b:=b); auto.
       eauto.
     Qed.
 
     Lemma p_halts_halt_with:
-      forall b,
-      PHalts (halt_with b).
+      forall b i,
+      PHalts (halt_with b) i.
     Proof.
       intros.
       apply p_halts_def with (r:=if b then Accept else Reject).
@@ -1443,11 +1507,11 @@ Require Import Coq.Logic.Classical_Prop.
       - destruct b; intros N; inversion N.
     Qed.
 
-    Definition PDecider (p:input->Prog) := forall i, PHalts (p i).
+    Definition PDecider (p:Prog) := forall i, PHalts p i.
 
     Lemma p_decider_def:
       forall p,
-      (forall i, PHalts (p i)) ->
+      (forall i, PHalts p i) ->
       PDecider p.
     Proof.
       intros.
@@ -1458,174 +1522,55 @@ Require Import Coq.Logic.Classical_Prop.
     Lemma p_decider_to_decider:
       forall p,
       PDecider p ->
-      Decider (Build p).
+      Decider p.
     Proof.
       intros.
       unfold Decider.
       intros.
       assert (H := H i).
-      destruct H as (r', (Hr,Hneq)).
-      apply run_build in Hr.
-      assert (r' = r) by eauto using exec_fun.
-      subst.
-      assumption.
+      apply H.
+    Qed.
+
+    Lemma p_halts_from_no_loop:
+      forall p i,
+      ~ Run p i Loop ->
+      PHalts p i.
+    Proof.
+      intros.
+      apply H.
     Qed.
 
     Lemma decider_to_p_decider:
       forall p,
-      Decider (Build (fun w => p w)) ->
+      Decider p ->
       PDecider p.
     Proof.
       unfold PDecider, Decider.
       intros.
       assert (H := H i).
-      destruct (exec_exists (Build (fun w : input => p w)) i) as (r, He).
-      assert (Hx := He).
-      apply H in He.
-      unfold PHalts.
-      apply run_build in Hx.
-      eauto.
+      auto using p_halts_from_no_loop.
     Qed.
 
     Lemma p_halts_seq_p_decider:
       forall p k,
       PDecider p ->
-      forall w,
-      (forall r b, Run (p w) r -> Dec r b -> PHalts (k b)) ->
-      PHalts (Seq (p w) k).
+      forall i,
+      (forall r b, Run p i r -> Dec r b -> PHalts (k b) i) ->
+      PHalts (Seq p k) i.
     Proof.
       intros.
       apply p_decider_to_decider in H.
-      apply decider_to_p_run with (w:=w) in H.
+      apply decider_to_p_run with (i:=i) in H.
       destruct H as (r, (b, (Hr, Hd))).
-      inversion Hr; subst; clear Hr.
       apply p_halts_seq with (r:=r) (b:=b); auto.
-      - apply run_build.
-        assumption.
-      - apply H0 with (r:=r).
-        + apply run_build. assumption.
-        + assumption.
+      eapply H0; eauto.
     Qed.
 
-    Definition PRecognizes (p:input->Prog) L : Prop :=
-      forall i, Run (p i) Accept <-> L i.
-
-    Lemma p_recognizes_def:
-      forall p (L:lang),
-      (forall i, Run (p i) Accept -> L i) ->
-      (forall i, L i -> Run (p i) Accept) ->
-      PRecognizes p L.
-    Proof.
-      intros.
-      unfold PRecognizes; intuition.
-    Qed.
-
-    Lemma p_recognizes_rw:
-      forall p L,
-      PRecognizes p L <-> Recognizes (Build p) L.
-    Proof.
-      intros.
-      unfold PRecognizes, Recognizes.
-      split; intros; split; intros.
-      - apply run_build in H0.
-        apply H.
-        assumption.
-      - apply run_build.
-        apply H.
-        assumption.
-      - apply run_build in H0.
-        apply H.
-        assumption.
-      - apply run_build.
-        apply H.
-        assumption.
-    Qed.
-
-    Lemma p_recognizable_def:
-      forall p L,
-      PRecognizes p L ->
-      Recognizable L.
-    Proof.
-      intros.
-      apply p_recognizes_rw in H.
-      eauto using recognizable_def.
-    Qed.
-
-    Lemma p_recognizes_run_reject:
-      forall p L i,
-      PRecognizes p L ->
-      Run (p i) Reject ->
-      ~ L i.
-    Proof.
-      intros.
-      rewrite p_recognizes_rw in H.
-      eapply recognizes_run_reject; eauto.
-      unfold Recognizes in H.
-      apply run_build in H0.
-      assumption.
-    Qed.
-
-
-    Lemma p_recognizes_run_loop:
-      forall p L i,
-      PRecognizes p L ->
-      Run (p i) Loop ->
-      ~ L i.
-    Proof.
-      intros.
-      rewrite p_recognizes_rw in H.
-      eapply recognizes_run_loop; eauto.
-      unfold Recognizes in H.
-      apply run_build in H0.
-      assumption.
-    Qed.
-
-    Lemma p_recognizes_run_accept:
-      forall p L i,
-      PRecognizes p L ->
-      Run (p i) Accept ->
-      L i.
-    Proof.
-      intros.
-      rewrite p_recognizes_rw in H.
-      eapply recognizes_run_accept; eauto.
-      unfold Recognizes in H.
-      apply run_build in H0.
-      assumption.
-    Qed.
-
-    Lemma p_recognizes_not_accept:
-      forall p L i r,
-      PRecognizes p L ->
-      Run (p i) r ->
-      ~ L i ->
-      r <> Accept.
-    Proof.
-      intros.
-      rewrite p_recognizes_rw in H.
-      apply run_build in H0.
-      eauto using recognizes_not_accept.
-    Qed.
-
-    Lemma p_recognizes_accept:
-      forall p L i r,
-      PRecognizes p L ->
-      Run (p i) r ->
-      L i ->
-      r = Accept.
-    Proof.
-      intros.
-      rewrite p_recognizes_rw in H.
-      apply run_build in H0.
-      assert (Exec (Build p) i Accept) by eauto using recognizes_accept.
-      eauto using exec_fun.
-    Qed.
-
-    Definition PDecides p L := PRecognizes p L /\ PDecider p.
+    Definition PDecides p L := Recognizes p L /\ PDecider p.
 
     Lemma p_decides_def:
       forall p L,
-      PRecognizes p L ->
+      Recognizes p L ->
       PDecider p ->
       PDecides p L.
     Proof.
@@ -1637,14 +1582,13 @@ Require Import Coq.Logic.Classical_Prop.
     Lemma p_decides_to_decides:
       forall p L,
       PDecides p L ->
-      Decides (Build p) L.
+      Decides p L.
     Proof.
       intros.
       unfold Decides.
       destruct H.
       split.
-      - apply p_recognizes_rw.
-        assumption.
+      - assumption.
       - apply p_decider_to_decider.
         assumption.
     Qed.
@@ -1652,7 +1596,7 @@ Require Import Coq.Logic.Classical_Prop.
     Lemma p_decides_to_p_recognizes:
       forall p L,
       PDecides p L ->
-      PRecognizes p L.
+      Recognizes p L.
     Proof.
       intros.
       destruct H.
@@ -1671,47 +1615,49 @@ Require Import Coq.Logic.Classical_Prop.
     Lemma p_decides_run_accept:
       forall p L i,
       PDecides p L ->
-      Run (p i) Accept ->
+      Run p i Accept ->
       L i.
     Proof.
       intros.
       apply p_decides_to_p_recognizes in H.
-      apply p_recognizes_run_accept with (p:=p); auto.
+      apply recognizes_run_accept with (p:=p); auto.
     Qed.
 
     Lemma p_decides_run_reject:
       forall p L i,
       PDecides p L ->
-      Run (p i) Reject ->
+      Run p i Reject ->
       ~ L i.
     Proof.
       intros.
       apply p_decides_to_p_recognizes in H.
-      eauto using p_recognizes_run_reject.
+      eauto using recognizes_run_reject.
     Qed.
 
     Lemma p_decider_run_dec:
       forall p i r,
       PDecider p ->
-      Run (p i) r ->
+      Run p i r ->
       exists b, Dec r b.
     Proof.
       intros.
       apply p_decider_to_decider in H.
-      apply run_build in H0.
-      eauto using neq_loop_to_dec.
+      apply neq_loop_to_dec.
+      intros N; subst.
+      unfold Decider in *.
+      apply H in H0; auto.
     Qed.
 
     Lemma p_decides_reject:
       forall p L i r,
       PDecides p L ->
-      Run (p i) r ->
+      Run p i r ->
       ~ L i ->
       r = Reject.
     Proof.
       intros.
       destruct H as (Ha, Hb).
-      apply p_recognizes_not_accept with (p:=p) (r:=r) in H1; auto.
+      apply recognizes_not_accept with (p:=p) in H1; auto.
       destruct r.
       - contradiction.
       - reflexivity.
@@ -1723,13 +1669,14 @@ Require Import Coq.Logic.Classical_Prop.
     Lemma p_decides_accept:
       forall p L i r,
       PDecides p L ->
-      Run (p i) r ->
+      Run p i r ->
       L i ->
       r = Accept.
     Proof.
       intros.
       apply p_decides_to_p_recognizes in H.
-      eauto using p_recognizes_accept.
+      eapply recognizes_accept in H1; eauto.
+      eauto using run_fun.
     Qed.
 
     Lemma p_decidable_def:
@@ -1742,44 +1689,16 @@ Require Import Coq.Logic.Classical_Prop.
       eauto using p_decides_to_decides.
     Qed.
 
-    Lemma recognizes_to_p_recognizes:
-      forall m L,
-      Recognizes m L ->
-      PRecognizes (fun w : input => Call m w) L.
-    Proof.
-      intros.
-      apply p_recognizes_def; intros.
-      - inversion H0; subst; clear H0.
-        apply recognizes_run_accept with (m:=m); auto.
-      - apply run_call.
-        apply recognizes_accept with (L:=L); auto.
-    Qed.
-
-    Lemma decider_to_p_decider_call:
-      forall m,
-      Decider m ->
-      PDecider (fun w : input => Call m w).
-    Proof.
-      intros.
-      apply p_decider_def.
-      intros.
-      auto using p_halts_call_decider.
-    Qed.
-
     Lemma decidable_to_p_decides:
       forall L,
       Decidable L ->
       exists p, PDecides p L.
     Proof.
       intros.
-      destruct H as (m, H).
-      exists (fun w => Call m w).
-      apply p_decides_def.
-      - apply decides_to_recognizes in H.
-        apply recognizes_to_p_recognizes.
-        assumption.
-      - apply decides_to_decider in H.
-        auto using decider_to_p_decider_call.
+      destruct H as (d, H).
+      exists d.
+      destruct H as (Ha, Hb).
+      auto using p_decides_def, decider_to_p_decider.
     Qed.
   End P_DECIDER.
 
@@ -1814,8 +1733,9 @@ Require Import Coq.Logic.Classical_Prop.
   Proof.
     unfold IsEmpty, NeverAccept; split; intros.
     - intros N; subst.
-      apply H in H0.
-      contradiction.
+      apply H in N.
+      unfold Empty in *.
+      assumption.
     - unfold Recognizes.
       split; intros. {
         apply H in H0.
@@ -1830,8 +1750,10 @@ Require Import Coq.Logic.Classical_Prop.
   match goal with
   | [ H: _ |- _ ] =>
     match type of H with
-      | Run (Call _ _) _ => idtac
-      | Run (Ret _) _ => idtac
+      | Run (With _ _) _ _ => idtac
+      | Run (Read _) _ _ => idtac
+      | Run (Call _) _ _ => idtac
+      | Run (Ret _) _ _ => idtac
       | Dec _ true => idtac
       | Dec _ false => idtac
       | Dec Accept _ => idtac
@@ -1862,40 +1784,35 @@ Require Import Coq.Logic.Classical_Prop.
     end.
 
   Ltac run_simpl_rw := (
-      rewrite decode_encode_machine_input_rw in * ||
+      rewrite decode_encode_prog_input_rw in * ||
       rewrite decode_encode_pair_rw in * ||
       rewrite encode_decode_pair_rw in * ||
-      rewrite decode_encode_machine_rw in * ||
-      rewrite encode_decode_machine_rw in *).
+      rewrite decode_encode_prog_rw in * ||
+      rewrite encode_decode_prog_rw in *).
+
 
   Ltac run_simpl_norm :=
     match goal with
-    | [ H: Loop = Accept |- _ ] => inversion H
-    | [ H: Loop = Reject |- _ ] => inversion H
-    | [ H: Accept = Loop |- _ ] => inversion H
-    | [ H: Accept = Reject |- _ ]  => inversion H
-    | [ H: Reject = Loop |- _ ] => inversion H
-    | [ H: Reject = Accept |- _ ] => inversion H
     | [ H: ?x = ?x |- _] => clear H
-    | [ H: Lang (Build _) _ |- _ ] => apply run_build in H
+    | [ H1: Run ?m ?i ?r1, H2: Run ?m ?i ?r2  |- _] =>
+      assert (r1 = r2) by eauto using run_fun;
+      subst; clear H1
     | [ H1: Exec ?m ?i ?r1, H2: Exec ?m ?i ?r2  |- _] =>
       assert (r1 = r2) by eauto using exec_fun;
       subst; clear H1
-    | H: Exec (Build _) _ _ |- _ => apply run_build in H
-    | [ H: _ |- Exec (Build _) _ _ ] => apply run_build
-    | [ H: Run (halt_with _) _ |- _ ] => apply run_halt_with_to_dec in H
-    | [ H: negb _ = true |- _ ] => apply negb_true_iff in H
-    | [ H: andb _ _ = true |- _] => apply andb_prop in H
-    | [ H: _ /\ _ |- _ ] => destruct H
-    | [ H: negb _ = false |- _ ] => apply negb_false_iff in H
-    | [ H: neg _ = Accept |- _ ] => apply neg_accept_rw in H
-    | [ H: neg _ = Reject |- _ ] => apply neg_reject_rw in H
-    | [ H: neg _ = Loop |- _ ] => apply neg_loop_rw in H
+    | [ H: Run (halt_with _) _ _ |- _ ] => apply run_halt_with_to_dec in H
     | [ H: true = _ |- _ ] => symmetry in H
     | [ H: false = _ |- _ ] => symmetry in H
     | [ H: Reject = _ |- _ ] => symmetry in H
     | [ H: Loop = _ |- _ ] => symmetry in H
     | [ H: Accept = _ |- _ ] => symmetry in H
+    | [ H: negb _ = true |- _ ] => apply negb_true_iff in H; subst
+    | [ H: negb _ = false |- _ ] => apply negb_false_iff in H; subst
+    | [ H: andb _ _ = true |- _] => apply andb_prop in H
+    | [ H: _ /\ _ |- _ ] => destruct H
+    | [ H: neg _ = Accept |- _ ] => apply neg_accept_rw in H
+    | [ H: neg _ = Reject |- _ ] => apply neg_reject_rw in H
+    | [ H: neg _ = Loop |- _ ] => apply neg_loop_rw in H
     end.
 
   Ltac run_simpl :=
